Add permissions to mapsto

theories/L7/L6_to_Clight_stack.v
@@ -1169,11 +1169,12 @@ Qed.
 Definition address := (block * Z)%type.
 
 Inductive mpred :=
-| Mapsto (bo : address) (vs : list Values.val)
+(* TODO technically could be a derived form *)
+| Mapsto (bo : address) (p : permission) (vs : list Values.val)
 | Sepcon (P Q : mpred)
 | Exists {A} (F : A -> mpred)
 | Mem (m : mem).
-Infix "↦" := Mapsto (at level 77).
+Notation "bo '↦_{' p '}' vs" := (Mapsto bo p vs) (at level 77).
 Infix "⋆" := Sepcon (at level 78, right associativity).
 Notation "'∃' x .. y , p" :=
   (Exists (fun x => .. (Exists (fun y => p)) ..))
@@ -1190,7 +1191,8 @@ Definition dom_mapsto (b : block) (o : Z) (vs : list Values.val) :=
 Reserved Notation "m |=_{ S } P" (at level 79).
 Fixpoint mpred_denote_aux (P : mpred) (S : Ensemble address) (m : mem) : Prop :=
   match P with
-  | (b, o) ↦ vs =>
+  | (b, o) ↦_{p} vs =>
+    Mem.range_perm m b o (o + #|vs|*word_size) Cur p /\
     S <--> dom_mapsto b o vs /\
     All (map val_wf vs) /\
     (forall i v, get_ith vs i = Some v -> load m b (o + i*word_size) = Some v) /\
@@ -1312,15 +1314,16 @@ Proof.
   + specialize (H b1 o1); subst; cbn in *; superlia.
 Qed.
 
-Lemma mapsto_app S b o vs ws m :
-  m |=_{S} ((b, o) ↦ vs ++ ws)%list <->
-  m |=_{S} ((b, o) ↦ vs) ⋆ ((b, o + #|vs|*word_size) ↦ ws)%Z.
+Lemma mapsto_app S b o p vs ws m :
+  m |=_{S} ((b, o) ↦_{p} vs ++ ws)%list <->
+  m |=_{S} ((b, o) ↦_{p} vs) ⋆ ((b, o + #|vs|*word_size) ↦_{p} ws)%Z.
 Proof.
   unfold mpred_denote_aux; split.
-  - intros [Hdom [Hwf [Hloads Hbounds]]].
+  - intros [Hperm [Hdom [Hwf [Hloads Hbounds]]]].
     rewrite dom_mapsto_app, map_app, All_app, app_length in *.
     do 2 eexists; split; [eassumption|].
-    split_ands; try (sets||tauto||cbn in *; superlia).
+    split_ands; try (sets||tauto||cbn in *; superlia||
+                     unfold Mem.range_perm in *; intros o' Ho'; apply Hperm; superlia).
     + rewrite dom_mapsto_Disjoint_simpl; superlia.
     + intros i v Hget.
       apply Hloads; rewrite <- Hget.
@@ -1332,33 +1335,43 @@ Proof.
       apply get_ith_range in Hget'.
       rewrite get_ith_suffix by lia.
       rewrite <- Hget; f_equal; lia.
-  - intros [S1 [S2 [HS [HD [[HS1 [Hwf1 [Hload1 Hbound1]]] [HS2 [Hwf2 [Hload2 Hbound2]]]]]]]].
+  - intros [S1 [S2 [HS [HD [[Hperm1 [HS1 [Hwf1 [Hload1 Hbound1]]]]
+                            [Hperm2 [HS2 [Hwf2 [Hload2 Hbound2]]]]]]]]].
     rewrite dom_mapsto_app, map_app, All_app, app_length, HS, HS1, HS2 in *.
     split_ands; try (sets||tauto||cbn in *; superlia).
-    intros i v Hget.
-    assert (Hcases : ((0 <= i < #|vs|) \/ (#|vs| <= i < #|vs| + #|ws|))%Z).
-    { apply get_ith_range in Hget. rewrite app_length in Hget. lia. }
-    destruct Hcases as [Hprefix|Hsuffix].
-    + apply Hload1; rewrite <- Hget, get_ith_prefix by lia; auto.
-    + replace (o + i*word_size)%Z with (o + #|vs|*word_size + (i-#|vs|)*word_size)%Z by lia.
-      apply Hload2; rewrite <- Hget, get_ith_suffix by lia; auto.
+    + unfold Mem.range_perm in *; intros o' Ho'.
+      specialize (Hperm1 o'); specialize (Hperm2 o').
+      match type of Hperm1 with ?t1 -> _ =>
+      match type of Hperm2 with ?t2 -> _ =>
+        assert (Hcases : t1 \/ t2) by superlia
+      end end.
+      destruct Hcases; eauto.
+    + intros i v Hget.
+      assert (Hcases : ((0 <= i < #|vs|) \/ (#|vs| <= i < #|vs| + #|ws|))%Z).
+      { apply get_ith_range in Hget. rewrite app_length in Hget. lia. }
+      destruct Hcases as [Hprefix|Hsuffix].
+      * apply Hload1; rewrite <- Hget, get_ith_prefix by lia; auto.
+      * replace (o + i*word_size)%Z with (o + #|vs|*word_size + (i-#|vs|)*word_size)%Z by lia.
+        apply Hload2; rewrite <- Hget, get_ith_suffix by lia; auto.
 Qed.
 
-Lemma mapsto_cons S b o v vs m :
-  m |=_{S} ((b, o) ↦ v :: vs) <->
-  m |=_{S} ((b, o) ↦ [v]) ⋆ ((b, o + word_size) ↦ vs)%Z.
+Lemma mapsto_cons S b o p v vs m :
+  m |=_{S} ((b, o) ↦_{p} v :: vs) <->
+  m |=_{S} ((b, o) ↦_{p} [v]) ⋆ ((b, o + word_size) ↦_{p} vs)%Z.
 Proof. apply mapsto_app with (vs := [v]). Qed.
 
-Lemma mapsto_store S b o i v vs m m' :
+Lemma mapsto_store S b o p i v vs m m' :
   val_wf v ->
   (0 <= i < #|vs|)%Z ->
   store m b (o + i*word_size) v = Some m' ->
-  m |=_{S} ((b, o) ↦ vs) ->
-  m' |=_{S} ((b, o) ↦ set_ith vs i v).
+  m |=_{S} ((b, o) ↦_{p} vs) ->
+  m' |=_{S} ((b, o) ↦_{p} set_ith vs i v).
 Proof.
   unfold mpred_denote_aux.
-  intros Hwf_v Hbound Hstore [HS [Hwf_vs [Hload Hbounds]]].
+  intros Hwf_v Hbound Hstore [Hperm [HS [Hwf_vs [Hload Hbounds]]]].
   split_ands; try (cbn in *; superlia).
+  - unfold Mem.range_perm in *; rewrite set_ith_len; intros o' Ho'.
+    eapply Mem.perm_store_1; eauto.
   - rewrite HS; clear; revert i o; induction vs as [|v' vs IHvs]; [easy|intros i o].
     cbn; destruct (Z.eq_dec i 0) as [|Hne]; [subst|].
     + apply Ensemble_iff_In_iff; intros [b' o'].
@@ -1385,12 +1398,18 @@ Lemma mpred_unchanged_on S P m m' :
   m |=_{S} P ->
   m' |=_{S} P.
 Proof.
-  revert S; induction P as [[b o] vs|P IHP Q IHQ|A F IHF|m'']; cbn;
+  revert S; induction P as [[b o] p vs|P IHP Q IHQ|A F IHF|m'']; cbn;
   intros S Hunchanged Hm.
-  - destruct Hm as [?[?[Hload [??]]]]; split_ands; auto.
-    intros i v Hget; eapply Mem.load_unchanged_on; eauto.
-    intros o'; cbn; rewrite Ensemble_iff_In_iff in H.
-    specialize (H (b, o')); rewrite H; unfold In, dom_mapsto; superlia.
+  - destruct Hm as [Hperm[HS[?[Hload [??]]]]]; split_ands; auto.
+    + destruct Hunchanged as [Hle Hperm' Haccess]; intros o' Ho'.
+      apply Hperm'; auto.
+      * rewrite Ensemble_iff_In_iff in HS; rewrite HS.
+        unfold dom_mapsto, In; lia.
+      * eapply Mem.perm_valid_block.
+        apply Hperm; eauto.
+    + intros i v Hget; eapply Mem.load_unchanged_on; eauto.
+      intros o'; cbn; rewrite Ensemble_iff_In_iff in HS.
+      specialize (HS (b, o')); rewrite HS; unfold In, dom_mapsto; superlia.
   - destruct Hm as [S1[S2[HS[?[??]]]]]; do 2 eexists; split_ands; eauto.
     + apply IHP; auto. 
       eapply Mem.unchanged_on_implies; eauto; cbn; intros; now apply (proj2 HS).
@@ -1401,15 +1420,15 @@ Proof.
     eapply Mem.unchanged_on_trans; eauto.
 Qed.
 
-Lemma mapsto_store_sepcon S P b o i v vs m m' :
+Lemma mapsto_store_sepcon S P b o p i v vs m m' :
   val_wf v ->
   (0 <= i < #|vs|)%Z ->
   store m b (o + i*word_size) v = Some m' ->
-  m |=_{S} ((b, o) ↦ vs) ⋆ P ->
-  m' |=_{S} ((b, o) ↦ set_ith vs i v) ⋆ P.
+  m |=_{S} ((b, o) ↦_{p} vs) ⋆ P ->
+  m' |=_{S} ((b, o) ↦_{p} set_ith vs i v) ⋆ P.
 Proof.
-  remember ((b, o) ↦ vs) as bovs.
-  remember ((b, o) ↦ set_ith vs i v) as bovs'.
+  remember ((b, o) ↦_{p} vs) as bovs.
+  remember ((b, o) ↦_{p} set_ith vs i v) as bovs'.
   cbn; subst bovs bovs'; intros Hwf Hrange Hstore.
   intros [S1 [S2 [HS [HD [Hbovs HP]]]]]; exists S1, S2; split_ands; auto.
   - eapply mapsto_store; eauto.
@@ -1418,7 +1437,7 @@ Proof.
     2:{ rewrite (Disjoint_pair_simpl S1 S2) in HD.
         intros o'; specialize (HD b o').
         intros Hin_S1 Hin_S2; contradiction HD.
-        destruct Hbovs as [HS1 _].
+        destruct Hbovs as [Hperm [HS1 _]].
         rewrite Ensemble_iff_In_iff in HS1.
         specialize (HS1 (b, o')); rewrite HS1.
         unfold dom_mapsto, In.
@@ -1532,23 +1551,23 @@ Proof.
     now rewrite_entailment (fun H => P' ⋆ H) sepcon_comm.
 Qed.
 
-Lemma mpred_load S F b o i v vs m :
+Lemma mpred_load S F b o p i v vs m :
   is_frame F ->
   get_ith vs i = Some v ->
-  m |=_{S} F ((b, o) ↦ vs) ->
+  m |=_{S} F ((b, o) ↦_{p} vs) ->
   load m b (o + i*word_size) = Some v.
 Proof.
   intros HF Hget; revert S; induction HF; intros S Hm;
   cbn in Hm; decompose [ex and] Hm; eauto.
 Qed.
 
-Lemma mpred_store S F b o i v vs m m' :
+Lemma mpred_store S F b o p i v vs m m' :
   is_frame F ->
   val_wf v ->
   (0 <= i < #|vs|)%Z ->
   store m b (o + i*word_size) v = Some m' ->
-  m |=_{S} F ((b, o) ↦ vs) ->
-  m' |=_{S} F ((b, o) ↦ set_ith vs i v).
+  m |=_{S} F ((b, o) ↦_{p} vs) ->
+  m' |=_{S} F ((b, o) ↦_{p} set_ith vs i v).
 Proof.
   intros HF Hwf Hrange Hstore Hm; destruct HF.
   - eapply mapsto_store; eauto.
@@ -1773,6 +1792,19 @@ Proof.
   eapply mpred_free'; eauto.
 Qed.
 
+(* TODO
+Definition local_word b (v : Values.val) :=
+  ∃ m m', Mem m'
+  WITH Some m' = store (alloc_alone m 0 word_size) b 0 v
+  WITH b = Mem.nextblock m.
+
+Search Mem.store list.
+Definition local_words b (v : list Values.val) :=
+  ∃ m m', Mem m'
+  WITH Some m' = store (alloc_alone m 0 word_size) b 0 v
+  WITH b = Mem.nextblock m.
+*)
+
 Definition vint (z : Z) : Values.val :=
   if Archi.ptr64
   then Vlong (Int64.repr z)
@@ -1795,10 +1827,10 @@ Fixpoint shadow_stack
   match frame_addrs, root_addrs, cvss with
   | [], [], [] => mempty
   | (f_b, f_o) :: frame_addrs, (r_b, r_o) :: root_addrs, rs :: cvss =>
-    (f_b, O.unsigned f_o) ↦
+    (f_b, O.unsigned f_o) ↦_{Freeable}
       Vptr r_b (O.repr (O.unsigned r_o + #|rs|*word_size)) ::
       Vptr r_b r_o :: stack_top frame_addrs :: [] ⋆
-    (r_b, O.unsigned r_o) ↦ rs ⋆
+    (r_b, O.unsigned r_o) ↦_{Freeable} rs ⋆
     shadow_stack frame_addrs root_addrs cvss
   | _, _, _ => mpure False
   end.
@@ -1814,12 +1846,12 @@ Definition valid_mem
            args frame_addrs root_addrs cvss nalloc frame : mpred :=
   ∃ args_b args_o,
   (∃ old_alloc old_limit heap,
-   (tinfo_b, O.unsigned tinfo_o) ↦
+   (tinfo_b, O.unsigned tinfo_o) ↦_{Writable}
    (old_alloc :: old_limit :: heap ::
     Vptr args_b args_o :: stack_top frame_addrs :: vint nalloc :: [])) ⋆
-   (∃ free_space, (nursery_b, O.unsigned alloc_o) ↦ free_space
+   (∃ free_space, (nursery_b, O.unsigned alloc_o) ↦_{Writable} free_space
     WITH #|free_space| = (O.unsigned limit_o - O.unsigned alloc_o)/word_size)%Z ⋆
-  ((args_b, O.unsigned args_o) ↦ args) ⋆
+  ((args_b, O.unsigned args_o) ↦_{Writable} args) ⋆
   (shadow_stack frame_addrs root_addrs cvss) ⋆
   (∃ gc_heap, Mem gc_heap) ⋆
   frame.
@@ -1839,7 +1871,7 @@ Fixpoint has_shape m v cv :=
     | Ret (boxed t a) =>
       match! cv with Vptr b o in
       exists cvs,
-      ((b, O.unsigned o - word_size) ↦ vint (rep_boxed t a) :: cvs) ∈ m /\
+      ((b, O.unsigned o - word_size) ↦_{Readable} vint (rep_boxed t a) :: cvs) ∈ m /\
       Forall2' (has_shape m) vs cvs
     | _ => False
     end
@@ -1861,8 +1893,8 @@ Fixpoint compatible_shape m m' v cv cv' :=
       match! cv with Vptr b o in
       match! cv' with Vptr b' o' in
       exists cvs cvs',
-      ((b, O.unsigned o - word_size) ↦ vint (rep_boxed t a) :: cvs) ∈ m /\
-      ((b', O.unsigned o' - word_size) ↦ vint (rep_boxed t a) :: cvs') ∈ m' /\
+      ((b, O.unsigned o - word_size) ↦_{Readable} vint (rep_boxed t a) :: cvs) ∈ m /\
+      ((b', O.unsigned o' - word_size) ↦_{Readable} vint (rep_boxed t a) :: cvs') ∈ m' /\
       Forall3 (compatible_shape m m') vs cvs cvs'
     | _ => False
     end
@@ -1956,7 +1988,7 @@ Definition rel_val_aux (k : nat) :=
     | Ret (boxed t a) =>
       match! cv with Vptr b o in
       exists cvs,
-      ((b, O.unsigned o - word_size) ↦ vint (rep_boxed t a) :: cvs) ∈ m /\
+      ((b, O.unsigned o - word_size) ↦_{Readable} vint (rep_boxed t a) :: cvs) ∈ m /\
       Forall2' (fun v cv => go v m cv) vs cvs
     | _ => False
     end%Z
